Add product bag [wip]

src/BinEncoders/take3/Base.v
@@ -2,16 +2,31 @@ Require Export List.
 
 Definition bin := list bool.
 
+Record encode_decode_R {A : Type} :=
+  { encode_R : A -> (bin -> bin) -> bin;
+    decode_R : forall B, bin -> (A -> bin -> B) -> B;
+    proof_R  : forall data encode data ( ) =              }.
+
 Section Specifications.
 
   Context {A : Type}.
-
   Variable predicate : A -> Prop.
   Variable encode : A -> bin.
-  Variable decode : bin -> A * bin.
+  Variable decode : bin -> A.
+  bin -> nat.
+
+  decode (encode a) = a
+
+  length (decode' (encode a ++ ext)) = length (encode a)
 
   Definition encode_correct :=
     forall val ext, predicate val -> decode ((encode val) ++ ext) = (val, ext).
+
+  Definition decode_shorten :=
+    forall ls, length (snd (decode ls)) <= pred (length ls).
+
+  Definition encode_nonnil :=
+    forall val, encode val <> nil.
 
 End Specifications.
 
@@ -19,5 +34,13 @@ Record encode_decode_R {A : Type} :=
   { predicate_R : A -> Prop;
     encode_R    : A -> bin;
     decode_R    : bin -> A * bin;
-    proof_R     : encode_correct predicate_R encode_R decode_R }.
+    proof_R     : encode_correct predicate_R encode_R decode_R;
+    shorten_R   : decode_shorten decode_R }.
+
+encode forall A B, A -> (bin -> B) -> B
+decode forall A B, bin -> (A -> bin -> B) -> B
+
+forall k a, encode a (\b. decode b k) = k a
+
+
 Arguments encode_decode_R : clear implicits.
