src/BinEncoders/take3/Char.v
@@ -1,11 +1,13 @@
-Require Import FixInt Ascii BinNat Omega Fiat.BinEncoders.Base.
+Require Import Fiat.BinEncoders.FixInt Ascii BinNat Omega Fiat.BinEncoders.Base.
 
 Section Char.
 
-  Definition encode c := encode_R (FixInt_encode_decode 8) (N_of_ascii c).
+  Lemma nonzero_8 : 0 < 8. omega. Qed.
+
+  Definition encode c := encode_R (FixInt_encode_decode 8 nonzero_8) (N_of_ascii c).
 
   Definition decode b :=
-    let (n, ext) := decode_R (FixInt_encode_decode 8) b
+    let (n, ext) := decode_R (FixInt_encode_decode 8 nonzero_8) b
     in (ascii_of_N n, ext).
 
   Lemma N_of_ascii_size : forall c, (N_of_ascii c < exp2 8)%N.
@@ -21,13 +23,21 @@ Section Char.
   Proof.
     unfold encode_correct, encode, decode.
     intros c ext _.
-    rewrite (proof_R (FixInt_encode_decode 8) _ _ (N_of_ascii_size _)).
+    rewrite (proof_R (FixInt_encode_decode 8 nonzero_8) _ _ (N_of_ascii_size _)).
     rewrite ascii_N_embedding. reflexivity.
+  Qed.
+
+  Theorem decode_shorten : decode_shorten decode.
+  Proof.
+    unfold decode_shorten, decode; intro ls.
+    pose proof (shorten_R (FixInt_encode_decode 8 nonzero_8) ls).
+    destruct (decode_R (FixInt_encode_decode 8 nonzero_8) ls); eauto.
   Qed.
 
   Definition Char_encode_decode :=
     {| predicate_R := fun _ => True;
        encode_R    := encode;
        decode_R    := decode;
-       proof_R     := encode_correct |}.
+       proof_R     := encode_correct;
+       shorten_R   := decode_shorten |}.
 End Char.
